06: add Church-Rosser draft

tapl/tapl/s05lambdaCalculus.lean
@@ -37,6 +37,7 @@
 import Mathlib.Data.Countable.Basic
 import Mathlib.Data.Finset.Basic
 import Mathlib.Data.Finset.Card
+import Mathlib.Data.Finset.Max
 import Mathlib.Logic.Relation
 
 namespace LambdaCalculus
@@ -53,12 +54,12 @@ def lid := LTerm.Abs (.Var 0)
 def tru :=
   LTerm.Abs
     (.Abs
-      (.Var 0))
+      (.Var 1))
 
 def fls :=
   LTerm.Abs
     (.Abs
-      (.Var 1))
+      (.Var 0))
 
 def test :=
   LTerm.Abs
@@ -66,17 +67,17 @@ def test :=
       (.Abs
         (.App
           (.App
-            (.Var 0)
+            (.Var 2)
             (.Var 1))
-          (.Var 2))))
+          (.Var 0))))
 
 def land :=
   LTerm.Abs
     (.Abs
       (.App
         (.App
-          (.Var 0)
-          (.Var 1))
+          (.Var 1)
+          (.Var 0))
         fls))
 
 def lor :=
@@ -84,9 +85,9 @@ def lor :=
     (.Abs
       (.App
         (.App
-          (.Var 0)
+          (.Var 1)
           tru)
-        (.Var 1)))
+        (.Var 0)))
 
 def lnot :=
   LTerm.Abs
@@ -102,8 +103,8 @@ def lpair :=
       (.Abs
         (.App
           (.App
-            (.Var 2)
-            (.Var 0))
+            (.Var 0)
+            (.Var 2))
           (.Var 1))))
 
 def fst :=
@@ -121,7 +122,7 @@ def snd :=
 def c0 :=
   LTerm.Abs
     (.Abs
-      (.Var 1))
+      (.Var 0))
 
 def scc :=
   LTerm.Abs
@@ -131,9 +132,9 @@ def scc :=
           (.Var 1)
           (.App
             (.App
-              (.Var 0)
+              (.Var 2)
               (.Var 1))
-            (.Var 2)))))
+            (.Var 0)))))
 
 --5.2.2
 def my_scc :=
@@ -142,11 +143,11 @@ def my_scc :=
       (.Abs
         (.App
           (.App
-            (.Var 0)
+            (.Var 2)
             (.Var 1))
           (.App
             (.Var 1)
-            (.Var 2)))))
+            (.Var 0)))))
 
 def plus :=
   LTerm.Abs
@@ -155,23 +156,23 @@ def plus :=
         (.Abs
           (.App
             (.App
-              (.Var 0)
-              (.Var 2))
+              (.Var 3)
+              (.Var 1))
             (.App
               (.App
-                (.Var 1)
-                (.Var 2))
-              (.Var 3))))))
+                (.Var 2)
+                (.Var 1))
+              (.Var 0))))))
 
 def times :=
   LTerm.Abs
     (.Abs
       (.App
         (.App
-          (.Var 0)
+          (.Var 1)
           (.App
             plus
-            (.Var 1)))
+            (.Var 0)))
         c0))
 
 --5.2.3
@@ -179,8 +180,8 @@ def my_times :=
   LTerm.Abs
     (.Abs
       (.App
-        (.Var 0)
-        (.Var 1)))
+        (.Var 1)
+        (.Var 0)))
 
 end Programming
 
@@ -224,9 +225,9 @@ class Infinite (α : Type) [DecidableEq α] where
 def subst [DecidableEq α] [Infinite α] : Term α → α → Term α → Term α
 | .Var x, f, s => if x = f then s else .Var x
 | .Abs x t, f, s =>
+  let y := Infinite.pick (FV t ∪ FV s ∪ {f})
   if x = f then .Abs x t
   else if x ∈ FV s then
-    let y := Infinite.pick (FV t ∪ FV s ∪ {f})
     .Abs y (subst (rename t x y) f s)
   else .Abs x (subst t f s)
 | .App t1 t2, f, s => .App (subst t1 f s) (subst t2 f s)
@@ -238,6 +239,7 @@ decreasing_by
 
 inductive AlphaRename [DecidableEq α] : Term α → Term α → Prop
 | rename : y ∉ FV t → AlphaRename (.Abs x t) (.Abs y (rename t x y))
+| self : AlphaRename t t
 
 inductive CompatClosure (R : Term α → Term α → Prop) : Term α → Term α → Prop
 | rel : R t t' → CompatClosure R t t'
@@ -246,7 +248,7 @@ inductive CompatClosure (R : Term α → Term α → Prop) : Term α → Term α
 | appR : CompatClosure R s s' → CompatClosure R (.App t s) (.App t s')
 
 def AlphaEq [DecidableEq α] : Term α → Term α → Prop :=
-  Relation.EqvGen (CompatClosure AlphaRename)
+  (CompatClosure AlphaRename)
 
 infix:50 " ~a " => AlphaEq
 
@@ -255,22 +257,269 @@ def a_term_setoid [DecidableEq α] : Setoid (Term α)  :=
 
 def ATerm (α : Type) [DecidableEq α] := Quotient (@a_term_setoid α _)
 
+lemma compat_closure_size (t t' : Term α) [DecidableEq α] :
+  CompatClosure AlphaRename t t' → size t = size t' := by
+    intro h
+    unhygienic induction h <;> grind [size, AlphaRename, rename_size_eq]
+
+lemma rename_self (t : Term α) (x : α) [DecidableEq α] :
+  rename t x x = t := by
+    induction t <;> grind [rename]
+
+lemma compat_trans (t1 t2 t3 : Term α) :
+  CompatClosure R t1 t2 → CompatClosure R t2 t3 → CompatClosure R t1 t3 := by
+    intro h1 h2
+    unhygienic induction t1 generalizing t2 t3
+    { cases h1
+      sorry }
+    { cases h1
+      { sorry }
+      cases h2
+      { sorry }
+      sorry }
+    sorry
+
+lemma compat_symm (t1 t2 : Term α) :
+  CompatClosure R t1 t2 → CompatClosure R t2 t1 := by
+    sorry
+
+lemma rename_rename (t : Term α) (x y : α) [DecidableEq α] :
+  x ∉ FV t → rename t x y ~a t := by
+    intro hx
+    unhygienic induction t
+    { simp only [rename]
+      split
+      { grind [FV] }
+      apply CompatClosure.rel
+      apply AlphaRename.self }
+    { simp only [rename]
+      split
+      { apply CompatClosure.rel
+        apply AlphaRename.self }
+      have : x ∉ FV t_1 := by grind [FV]
+      apply CompatClosure.abs
+      aesop }
+    rw [rename]
+    apply compat_trans
+    { apply CompatClosure.appL
+      apply t1_ih (by grind [FV]) }
+    apply CompatClosure.appR
+    exact t2_ih (by grind [FV])
+
+lemma rename_FV (t : Term α) (x y : α) [DecidableEq α] :
+  ∀ a, a ∈ FV (rename t x y) → a ∈ FV t ∧ a ≠ x ∨ a = y ∧ x ∈ FV t := by
+    unhygienic induction t <;> grind [FV, rename]
+
+lemma induction_size_specified (P : Term α → Prop) :
+  ∀ gen_sz, (∀ (s : Term α), (∀ r, size r < size s → P r) → P s) → ∀ s, size s < gen_sz  → P s := by
+    intro gen_sz ind s hlt
+    induction gen_sz generalizing s <;> grind
+
+
+lemma induction_size (P : Term α → Prop) :
+  (∀ s, (∀ r, size r < size s → P r) → P s) → ∀ t, P t := by
+  intro ind s
+  exact induction_size_specified P (size s + 1) ind s (by simp)
+
+lemma subst_fv (t : Term α) (f : α) (s : Term α) [DecidableEq α] [Infinite α] :
+  f ∉ FV t → t ~a subst t f s := by
+    apply induction_size (P := fun t => f ∉ FV t → t ~a subst t f s)
+    intro t ind hn
+    unhygienic cases t
+    { rw [subst]
+      have : x ≠ f := by grind [FV]
+      rw [if_neg this]
+      apply CompatClosure.rel
+      apply AlphaRename.self }
+    { rw [subst]
+      repeat' split
+      { apply CompatClosure.rel
+        apply AlphaRename.self}
+      { simp [FV] at hn
+        have lms :=
+          AlphaRename.rename (t := t_1) (x := x) (y := Infinite.pick (FV t_1 ∪ FV s ∪ {f}))
+            (by grind [Infinite.pick_is_fresh])
+        apply compat_trans
+        { apply CompatClosure.rel
+          apply lms }
+        apply CompatClosure.abs
+        apply ind (rename t_1 x (Infinite.pick (FV t_1 ∪ FV s ∪ {f})))
+          (by grind [size, rename_size_eq])
+        intro hts
+        have st := rename_FV t_1 x (Infinite.pick (FV t_1 ∪ FV s ∪ {f})) f hts
+        grind [Infinite.pick_is_fresh] }
+      apply CompatClosure.abs
+      apply ind t_1 (by simp [size])
+      grind [FV] }
+    rw [subst]
+    apply compat_trans
+    { apply CompatClosure.appL
+      apply ind t1 (by grind [size]) (by grind [FV]) }
+    apply CompatClosure.appR
+    apply ind t2 (by grind [size]) (by grind [FV])
+
 lemma subst_respects_alpha [DecidableEq α] [Infinite α]
   {t t' : Term α} {f : α} {s : Term α} :
   t ~a t' → (subst t f s) ~a (subst t' f s) := by
-  intro ha
-  induction ha
-  · rename_i h
-    cases h
-    · sorry
-    · sorry
-    · sorry
-    · sorry
-  · apply Relation.EqvGen.refl
-  · apply Relation.EqvGen.symm
-    assumption
-  · apply Relation.EqvGen.trans
-    repeat assumption
+  apply induction_size (P := fun t => ∀ t', t ~a t' → (subst t f s) ~a (subst t' f s))
+  intro t ind t' ha
+  unhygienic cases t
+  { unhygienic cases ha
+    cases a
+    apply CompatClosure.rel
+    apply AlphaRename.self }
+  { unhygienic cases ha
+    { unhygienic cases a
+      { rw [subst]
+        split_ifs with h
+        { rw [subst]
+          split_ifs with h1
+          { apply CompatClosure.rel
+            apply AlphaRename.rename a_1 }
+          { apply compat_symm
+            apply compat_trans
+            { apply CompatClosure.abs
+              apply compat_symm
+              apply subst_fv _ f s
+              intro contra
+              unhygienic cases rename_FV _ _ _ f contra
+              { cases rename_FV _ _ _ f h_1.1 <;> grind }
+              grind [Infinite.pick_is_fresh] }
+            apply compat_trans
+            { apply compat_symm
+              apply CompatClosure.rel
+              apply AlphaRename.rename
+              intro contra
+              cases rename_FV _ _ _ _ contra <;> grind [Infinite.pick_is_fresh] }
+            apply compat_symm
+            apply CompatClosure.rel
+            apply AlphaRename.rename a_1 }
+          apply compat_trans
+          { apply CompatClosure.rel
+            apply AlphaRename.rename (y := y) a_1 }
+          apply CompatClosure.abs
+          apply subst_fv
+          intro contra
+          have := rename_FV t_1 x y f contra
+          grind }
+        { rw [subst]
+          split_ifs with h1
+          { apply compat_trans
+            { apply compat_symm
+              apply CompatClosure.abs
+              apply subst_fv
+              intro contra
+              cases rename_FV _ _ _ _ contra
+              { grind }
+              grind [Infinite.pick_is_fresh] }
+            apply compat_symm
+            apply compat_trans
+            { apply CompatClosure.rel
+              apply AlphaRename.rename (y := (Infinite.pick (FV t_1 ∪ FV s ∪ {f})))
+              intro contra
+              cases rename_FV _ _ _ _ contra <;> grind [Infinite.pick_is_fresh] }
+            apply compat_trans
+            { apply compat_symm
+              apply CompatClosure.rel
+              apply AlphaRename.rename
+              intro contra
+              cases rename_FV _ _ _ _ contra <;> grind [Infinite.pick_is_fresh] }
+            apply compat_symm
+            apply compat_trans
+            { apply compat_symm
+              apply CompatClosure.rel
+              apply AlphaRename.rename
+              grind [Infinite.pick_is_fresh] }
+            apply CompatClosure.rel
+            apply AlphaRename.rename
+            grind [Infinite.pick_is_fresh] }
+          { apply compat_trans
+            { apply CompatClosure.abs
+              stop sorry }
+            sorry }
+          stop sorry }
+        rw [subst]
+        split_ifs with h1 h2
+        stop sorry }
+      apply CompatClosure.rel
+      apply AlphaRename.self }
+    rw [subst, subst]
+    split_ifs with h1 h2
+    { apply CompatClosure.abs
+      apply a }
+    { apply compat_trans
+      { apply CompatClosure.rel
+        apply AlphaRename.rename (y := Infinite.pick (FV t_1 ∪ FV t'_1 ∪ FV s ∪ {f}))
+
+        sorry }
+      apply compat_symm
+      apply compat_trans
+      { apply CompatClosure.rel
+        apply AlphaRename.rename (y := Infinite.pick (FV t_1 ∪ FV t'_1 ∪ FV s ∪ {f}))
+        sorry }
+      apply CompatClosure.abs
+
+      have := ind t_1 (by grind [size]) t'_1 a
+      sorry }
+    apply CompatClosure.abs
+    apply ind t_1 (by grind [size]) t'_1 a }
+  rw [subst]
+  unhygienic cases ha
+  { cases a
+    rw [subst]
+    apply CompatClosure.rel
+    apply AlphaRename.self }
+  { rw [subst]
+    apply CompatClosure.appL
+    apply ind t1 (by grind [size])
+    exact a }
+  rw [subst]
+  apply CompatClosure.appR
+  apply ind t2 (by grind [size])
+  exact a
+  /-unhygienic induction ha
+  { unhygienic cases a
+    { rw [subst, subst]
+      repeat' unhygienic split
+      { rename_i h1 h2
+        rw [h1, h2, rename_self]
+        apply CompatClosure.rel
+        apply AlphaRename.self }
+      { sorry }
+      { sorry }
+      { sorry }
+      { sorry }
+      { sorry }
+      { sorry }
+      { sorry }
+      stop sorry }
+    apply CompatClosure.rel
+    apply AlphaRename.self }
+  { rw [subst, subst]
+    repeat' unhygienic split
+    { apply CompatClosure.abs
+      exact a }
+    { have y := Infinite.pick (FV t_1 ∪ FV s ∪ {f})
+      have st :
+        Term.Abs y (subst (rename t_1 x y) f s) =
+        Term.Abs y (rename (subst t_1 f s) x y) := by
+
+          sorry
+      have :
+        Term.Abs y (subst (rename t_1 x y) f s) ~a
+        Term.Abs y (subst t_1 f s) := by
+
+
+          sorry
+      sorry }
+    apply CompatClosure.abs
+    exact a_ih }
+  { rw [subst, subst]
+    apply CompatClosure.appL
+    exact a_ih }
+  rw [subst, subst]
+  apply CompatClosure.appR
+  exact a_ih-/
 
 def substA [DecidableEq α] [Infinite α]
   (t : ATerm α) (f : α) (s : Term α) : ATerm α :=
